\documentclass[12pt]{article}
\usepackage[margin=2.5cm]{geometry}
\usepackage{enumerate}
\usepackage{amsfonts}
\usepackage{amsmath}
\usepackage{fancyhdr}
\usepackage{amsmath}
\usepackage{amssymb}
\usepackage{amsthm}
\usepackage{mdframed}
\usepackage{graphicx}
\usepackage{subcaption}
\usepackage{adjustbox}
\usepackage{listings}
\usepackage{xcolor}
\usepackage{booktabs}
\usepackage[utf]{kotex}

\definecolor{codegreen}{rgb}{0,0.6,0}
\definecolor{codegray}{rgb}{0.5,0.5,0.5}
\definecolor{codepurple}{rgb}{0.58,0,0.82}
\definecolor{backcolour}{rgb}{0.95,0.95,0.92}

\lstdefinestyle{mystyle}{
    backgroundcolor=\color{backcolour},
    commentstyle=\color{codegreen},
    keywordstyle=\color{magenta},
    numberstyle=\tiny\color{codegray},
    stringstyle=\color{codepurple},
    basicstyle=\ttfamily\footnotesize,
    breakatwhitespace=false,
    breaklines=true,
    captionpos=b,
    keepspaces=true,
    numbers=left,
    numbersep=5pt,
    showspaces=false,
    showstringspaces=false,
    showtabs=false,
    tabsize=1
}

\lstset{style=mystyle}

\begin{document}
\title{CSC236 Worksheet 4 Review}
\author{Hyungmo Gu}
\maketitle

\section*{Question 1}
\begin{itemize}
    \item

    Let $n \in \mathbb{N}$. Assume that $\exists k \in \mathbb{N},\:n = 3^k$, so
    $k = \log_3 n$.

    \bigskip

    Then,

    \bigskip

    \begin{align}
        T(n) &= 2n + T(\lceil n/3 \rceil) & [\text{By def.}]\\
        &= 2n + T(n/3) & [\text{Since $3 \mid n$, and $\lceil n/3 \rceil = n/3$}]\\
        &= 2n + (2(n/3) + T(n/3^2)) & [\text{By subtituting $n/3$ for $n$ in def.}]\\
        &\vdots\\
        &=2n\sum\limits_{i=0}^{k-1} \frac{1}{3^i} + T(n/3^k) & [\text{After $k$ steps}]\\
        &=2n \Bigl( \frac{1 - (1/3^k)}{1 - (1/3)} \Bigr) + T(n/3^k) & [\text{By geometric series}]\\
        &=2 \cdot 3^k \Bigl( \frac{1 - (1/3^k)}{1 - (1/3)}  \Bigr) + T(3^k/3^k) & [\text{By replacing $3^k$ for $n$}]\\
        &=3(3^k - 1) + 2\\
        &=3^{k+1} - 1\\
        &=3^{\log_3 n + 1} - 1 & [\text{By replacing $\log_3 n$ for $k$}]\\
        &=3^{\log_3 n + \log_3 3} - 1\\
        &=3^{\log_3 3n} - 1\\
        &=3n - 1
    \end{align}

    \bigskip

    \begin{mdframed}
        \underline{\textbf{Attempt 2:}}

        \bigskip

        Let $n \in \mathbb{N}$. Assume that $\exists k \in \mathbb{N},\:n = 3^k$, so
        $k = \log_3 n$.

        \bigskip

        Then,

        \bigskip

        \begin{align}
            T(n) &= 2n + T(\lceil n/3 \rceil) & [\text{By def.}]\\
            &= 2n + T(n/3) & [\text{Since $3 \mid n$, and $\lceil n/3 \rceil = n/3$}]\\
            &= 2n + (2(n/3) + T(n/3^2)) & [\text{By \color{red}replacing\color{black}\:$n/3$ for $n$ in def.}]\\
            &\vdots\\
            &=2n\sum\limits_{i=0}^{k-1} \frac{1}{3^i} + T(n/3^k) & [\text{After $k$ steps}]\\
            &=2n \Bigl( \frac{1 - (1/3^k)}{1 - (1/3)} \Bigr) + T(n/3^k) & [\text{By geometric series}]\\
            &=2 \cdot 3^k \Bigl( \frac{1 - (1/3^k)}{1 - (1/3)}  \Bigr) + T(3^k/3^k) & [\text{By replacing $3^k$ for $n$}]\\
            &=3(3^k - 1) + 2\\
            &=3^{k+1} - 1\\
            &=3^{\log_3 n + 1} - 1 & [\text{By replacing $\log_3 n$ for $k$}]\\
            &=3^{\log_3 n + \log_3 3} - 1\\
            &=3^{\log_3 3n} - 1\\
            &=3n - 1
        \end{align}
    \end{mdframed}

    % \bigskip

    % \begin{mdframed}
    % \underline{\textbf{Rough Work:}}

    % \bigskip

    % Let $n \in \mathbb{N}$. Assume that $\exists k \in \mathbb{N},\:n = 3^k$, so
    % $k = \log_3 n$.

    % \bigskip

    % Then,

    % \bigskip

    % \begin{align}
    %     T(n) &= 2n + T(\lceil n/3 \rceil) & [\text{By def.}]\\
    %     &= 2n + T(n/3) & [\text{Since $3 \mid n$, and $\lceil n/3 \rceil = n/3$}]\\
    %     &= 2n + (2(n/3) + T(n/3^2)) & [\text{By subtituting $n/3$ for $n$ in def.}]\\
    %     &\vdots\\
    %     &=2n\sum\limits_{i=0}^{k-1} \frac{1}{3^i} + T(n/3^k) & [\text{After $k$ steps}]\\
    %     &=2n \Bigl( \frac{1 - (1/3^k)}{1 - (1/3)} \Bigr) + T(n/3^k) & [\text{By geometric series}]\\
    %     &=2 \cdot 3^k \Bigl( \frac{1 - (1/3^k)}{1 - (1/3)}  \Bigr) + T(3^k/3^k) & [\text{By replacing $3^k$ for $n$}]\\
    %     &=3(3^k - 1) + 2\\
    %     &=3^{k+1} - 1\\
    %     &=3^{\log_3 n + 1} - 1 & [\text{By replacing $\log_3 n$ for $k$}]\\
    %     &=3^{\log_3 n + \log_3 3} - 1\\
    %     &=3^{\log_3 3n} - 1\\
    %     &=3n - 1
    % \end{align}

    % \end{mdframed}
\end{itemize}

\end{document}