\documentclass[12pt]{article}
\usepackage{enumerate}
\usepackage{amsfonts}
\usepackage{amsmath}
\usepackage{fancyhdr}
\usepackage{mathtools}

\begin{document}
\title{Worksheet 3 Solution}
\maketitle

\section*{Question 1}

Part 1
\begin{enumerate}[a)]
    \item
        $Correct(my\_prog) \land Python(my\_prog)$
    \item
        $\exists x \in P,\: \neg Correct(x) \Rightarrow Python(x)$
    \item
        $\forall x \in P,\: \neg Python(x) \Rightarrow Correct(x)$
    \item
        $\forall x \in P,\: \neg Correct(x) \Rightarrow Correct(x)$
    \item
        A program is written in Python and is correct
    \item
        All programs are not written in Python and is correct
    \item
        It is not true that all programs written in python is correct
    \item
        All programs that are not written in python is correct, and all correctly running programs are not written in python

\end{enumerate}

\section*{Question 2}

\begin{enumerate}[a)]
    \item
        All program written in Python is correct, or all program written in Python is not correct
    \item
        $(\exists x \in P,\: Python(x) \Rightarrow Correct(x)) \Rightarrow (\forall y \in P, Python(x) \Rightarrow Correct(x))$
    \item
        The first statement considers two different natural numbers, where as the second uses the same number

        The first statement is True (with $x_1 = 5$ and $x_2 = 35$), but the second statement is False (165 cannot be in multiples of 7)
\end{enumerate}

\section*{Question 3}

\begin{enumerate}[a)]
    \item
        $Odd(x):\: \exists n \in \mathbb{Z},\: 2 \mid (n+1)$
    \item
        $(\forall m \in \mathbb{Z},\:Odd(m))\land(\forall n \in \mathbb{Z},\:Odd(n)) \Rightarrow Odd(mn)$
    \item
        $\forall m,n \in \mathbb{Z},\:\exists k,l \in \mathbb{Z},\:((m+1)=2k)\land((n+1)=2l) \Rightarrow \exists o \in \mathbb{Z}, (mn+1)=2o$
    \item
        $\forall m,n \in \mathbb{Z}, \exists k \in \mathbb{Z},\:((mn+1)=2k) \Rightarrow \exists l,o \in \mathbb{Z}, ((m+1)=2l)\land((n+1)=2o)$

\end{enumerate}


\section*{Question 4}
    \begin{enumerate}[a)]
        \item
        \begin{equation}
            \neg ((a \land b) \Leftrightarrow c)
        \end{equation}

        Expanding definition of iff:

        \begin{equation}
            \neg (((a\land b) \land c) \lor (\neg (a \land b) \land \neg c))
        \end{equation}

        Using $\neg(p \lor q) \Rightarrow \neg p \land \neg q$:

        \begin{equation}
            \neg((a\land b) \land c) \land \neg (\neg (a \land b) \land \neg c)
        \end{equation}

        Using $\neg(p \land q) \Rightarrow \neg p \lor \neg q$:

        \begin{equation}
            (\neg(a\land b) \lor \neg c) \land ((a \land b) \lor c)
        \end{equation}

        \item
        Using rule \#6 and \#7:

        \begin{equation}
            \exists x,y \in S,\: \forall z \in S,\:\neg (P(x,y) \land Q(x,z))
        \end{equation}

        Using rule \#2:

        \begin{equation}
            \exists x,y \in S,\: \forall z \in S,\:\neg P(x,y) \lor \neg Q(x,z)
        \end{equation}

    \end{enumerate}

\section*{Question 5}

\end{document}