\documentclass[12pt]{article}
\usepackage[margin=2.5cm]{geometry}
\usepackage{enumerate}
\usepackage{amsfonts}
\usepackage{amsmath}
\usepackage{fancyhdr}
\usepackage{amsmath}
\usepackage{amssymb}
\usepackage{amsthm}
\usepackage{mdframed}
\usepackage{graphicx}
\usepackage{subcaption}
\usepackage{adjustbox}
\usepackage{listings}
\usepackage{xcolor}
\usepackage{booktabs}
\usepackage[utf]{kotex}

\definecolor{codegreen}{rgb}{0,0.6,0}
\definecolor{codegray}{rgb}{0.5,0.5,0.5}
\definecolor{codepurple}{rgb}{0.58,0,0.82}
\definecolor{backcolour}{rgb}{0.95,0.95,0.92}

\lstdefinestyle{mystyle}{
    backgroundcolor=\color{backcolour},
    commentstyle=\color{codegreen},
    keywordstyle=\color{magenta},
    numberstyle=\tiny\color{codegray},
    stringstyle=\color{codepurple},
    basicstyle=\ttfamily\footnotesize,
    breakatwhitespace=false,
    breaklines=true,
    captionpos=b,
    keepspaces=true,
    numbers=left,
    numbersep=5pt,
    showspaces=false,
    showstringspaces=false,
    showtabs=false,
    tabsize=1
}

\lstset{style=mystyle}

\begin{document}
\title{CSC263 Worksheet 1 Solution}
\author{Hyungmo Gu}
\maketitle

\section*{Question 1}
\begin{enumerate}[a.]
    \item

    \begin{proof}
        Assume the statement $P(115)$ is true. That is, $\sum\limits_{i=0}^{i=115} 2^i = 2^{115+1}$.

        \bigskip

        We need to prove $\sum\limits_{i=0}^{i=116} 2^i = 2^{116+1}$.

        \bigskip

        Starting from the left, we can write

        \bigskip

        \begin{align}
            \sum\limits_{i=0}^{i=116} 2^i = \sum\limits_{i=0}^{i=115} 2^i + 2
        \end{align}

        \bigskip

        Then, using the assumption $\sum\limits_{i=0}^{i=115} 2^i = 2^{115+1}$, we
        can conclude

        \begin{align}
            \sum\limits_{i=0}^{i=116} 2^i &= 2^{115+1} + 2^{116}\\
            &= 2^{116} + 2^{116}\\
            &= 2^{116}(1 + 1)\\
            &= 2 \cdot 2^{116}\\
            &= 2^{116+1}
        \end{align}
    \end{proof}

    \item

    \begin{proof}
        No. The statement is not true for every natural natural number.

        \bigskip

        We will prove this by counter example. That is, $\exists n \in \mathbb{N},\:
        \sum\limits_{i=0}^{i=n} 2^i \neq 2^{n+1}$.

        \bigskip

        Let $n = 0$.

        \bigskip

        Then, starting from the left hand side, it follows from the fact $n = 0$ that

        \setcounter{equation}{0}
        \begin{align}
            \sum\limits_{i=0}^{i=n} 2^i &= \sum\limits_{i=0}^{i=0} 2^i\\
            &= 0
        \end{align}


        Now, for the right hand side, using the same fact, we can write

        \begin{align}
            2^{0+1} &= 2^1\\
            &= 2
        \end{align}
    \end{proof}

\end{enumerate}

\bigskip

\section*{Question 2}
\begin{itemize}
    \item

    \underline{\textbf{Statement:}} $\forall n \in \mathbb{N},\:\exists d \in \mathbb{Z},\:8^n-1 = 7d$

    \bigskip

    \begin{proof}

    We will prove this statement by induction on $n$.

    \bigskip

    \underline{\textbf{Base Case:}}

    \bigskip

    Let $n = 0$.

    \bigskip

    We need to prove $8^n-1 = 7 \cdot 0$.

    \bigskip

    Starting from the left hand side, using the fact $n = 0$, we can conclude,
    \setcounter{equation}{0}
    \begin{align}
        8^{0} - 1 &= 1 - 1\\
        &= 0\\
        &= 7 \cdot 0
    \end{align}

    \bigskip

    \underline{\textbf{Inductive Step:}}

    \bigskip

    Let $n \in \mathbb{N}$. Assume there is an integer $d$ such that $8^n-1 = 7d$.

    \bigskip

    We need to prove there is an integer $\tilde{d}$ such that $8^{n+1} - 1 = 7 \tilde{d}$.

    \bigskip

    Let $\tilde{d} = 8^n+d$.

    \bigskip

    Starting from the left hand side, we can write

    \bigskip
    \begin{align}
        8^{n+1} - 1 &= 8^n + 8^n + 8^n + 8^n + 8^n + 8^n + 8^n + 8^n - 1\\
        &= 8^n + 8^n + 8^n + 8^n + 8^n + 8^n + 8^n + (8^n - 1)
    \end{align}

    \bigskip

    Then, using inductive hypothesis, i.e. $8^n-1 = 7d$, we can conclude

    \begin{align}
        8^{n+1} - 1 &= 8^n + 8^n + 8^n + 8^n + 8^n + 8^n + 8^n + 7d\\
        &= 7 \cdot 8^n + 7d\\
        &= 7 \cdot (8^n + d)\\
        &= 7 \cdot \tilde{d}
    \end{align}

    \end{proof}

    % \bigskip

    % \begin{mdframed}
    %     \underline{\textbf{Rough Work:}}

    %     \bigskip

    %     \begin{enumerate}[1.]
    %         \item Base Case

    %         \begin{mdframed}
    %         \underline{\textbf{Base Case:}}

    %         \bigskip

    %         Let $n = 0$.

    %         \bigskip

    %         We need to prove $8^n-1 = 7 \cdot 0$.

    %         \bigskip

    %         Starting from the left hand side, using the fact $n = 0$, we can conclude,
    %         \setcounter{equation}{0}
    %         \begin{align}
    %             8^{0} - 1 &= 1 - 1\\
    %             &= 0\\
    %             &= 7 \cdot 0
    %         \end{align}

    %         \end{mdframed}

    %         \item Inductive Step

    %         \begin{mdframed}
    %         \underline{\textbf{Inductive Step:}}

    %         \bigskip

    %         Let $n \in \mathbb{N}$. Assume there is an integer $d$ such that $8^n-1 = 7d$.

    %         \bigskip

    %         We need to prove there is an integer $\tilde{d}$ such that $8^{n+1} - 1 = 7 \tilde{d}$.

    %         \bigskip

    %         Let $\tilde{d} = 8^n+d$.

    %         \bigskip

    %         Starting from the left hand side, we can write

    %         \bigskip
    %         \begin{align}
    %             8^{n+1} - 1 &= 8^n + 8^n + 8^n + 8^n + 8^n + 8^n + 8^n + 8^n - 1\\
    %             &= 8^n + 8^n + 8^n + 8^n + 8^n + 8^n + 8^n + (8^n - 1)
    %         \end{align}

    %         \bigskip

    %         Then, using inductive hypothesis, i.e. $8^n-1 = 7d$, we can conclude

    %         \begin{align}
    %             8^{n+1} - 1 &= 8^n + 8^n + 8^n + 8^n + 8^n + 8^n + 8^n + 7d\\
    %             &= 7 \cdot 8^n + 7d\\
    %             &= 7 \cdot (8^n + d)\\
    %             &= 7 \cdot \tilde{d}
    %         \end{align}

    %         \bigskip
    %         \end{mdframed}
    %     \end{enumerate}
    % \end{mdframed}
\end{itemize}

\section*{Question 3}

\section*{Question 4}

\end{document}