\documentclass[12pt]{article}
\usepackage{enumerate}
\usepackage{amsfonts}
\usepackage{amsmath}
\usepackage{fancyhdr}
\usepackage{amssymb}

\begin{document}
\title{Worksheet 5 Review}
\maketitle

\section*{Question 1}
\begin{itemize}
    \item

    \textbf{Predicate Logic:} $\forall x,y \in \mathbb{Z}, Odd(x) \land Odd(y)
    \Rightarrow Odd(xy)$

    \bigskip

    Let $x,y \in \mathbb{Z}$. Assume $Odd(x)$ and $Odd(y)$.

    \bigskip

    Then, $\exists k,m \in \mathbb{Z}$,

    \begin{align}
        x &= 2k - 1\\
        y &= 2m - 1
    \end{align}

    \bigskip

    Then,

    \begin{align}
        xy &= (2k-1)(2m-1)\\
        xy &= (4km - 2k - 2m + 2) - 1\\
        xy &= 2(2km - k - m + 1) - 1\\
        xy &= 2o - 1
    \end{align}

    by setting $o = 2km - k - m + 1$.

    \bigskip

    Since, $o \in \mathbb{Z}$, it follows from the definition of odd that the statement
    $\forall x,y \in \mathbb{Z}, Odd(x) \land Odd(y) \Rightarrow Odd(xy)$ is true.
\end{itemize}

\section*{Question 2}
\begin{enumerate}[a.]
    \item

    $\forall n,m \in \mathbb{Z},\:Even(n) \land Odd(m) \Rightarrow m^2 - n^2 = m + n$

    \item

    The flaw is that the value $k$ in $n = 2k$ and $m = 2k + 1$ cannot be the same.
\end{enumerate}
\section*{Question 3}
\begin{enumerate}[a.]
    \item

    $Dom(f,g): \forall n \in \mathbb{Z},\: g(n) \leq f(n)$, where $f,g: \mathbb{N}
    \to \mathbb{R}^{\geq 0}$
\end{enumerate}

\section*{Question 4}

\end{document}